# baseURI: https://example.org/sba-mpc-schema#
@prefix : <https://example.org/sba-mpc-schema#> .

@prefix sba: <https://example.org/sba-schema#> .
@prefix eva: <https://example.org/sba-eva-schema#> .
@prefix mpc: <https://example.org/sba-mpc-schema#> .
@prefix forc: <https://example.org/sba-forecast-schema#> .

@prefix sosa: <http://www.w3.org/ns/sosa/> .
@prefix wot: <https://www.w3.org/2019/wot/td/v1#> .
@prefix saref: <https://w3id.org/saref#> .
@prefix xsd: <http://www.w3.org/2001/XMLSchema#> .
@prefix td: <https://www.w3.org/2019/wot/td#> .
@prefix s3n: <http://w3id.org/s3n/> .
@prefix rdfs: <http://www.w3.org/2000/01/rdf-schema#> .
@prefix openadr: <https://w3id.org/def/openadr#> .
@prefix unit: <http://qudt.org/vocab/unit/> .
@prefix brick: <https://brickschema.org/schema/Brick#> .
@prefix ref: <https://brickschema.org/schema/Brick/ref#> .
@prefix bot: <https://w3id.org/bot#> .
@prefix ssn: <http://www.w3.org/ns/ssn/> .
@prefix rdf: <http://www.w3.org/1999/02/22-rdf-syntax-ns#> .

#################################################################
#     MPC Schema
#################################################################

#################################################################
#     Classes
#################################################################

mpc:EVMPC
  rdfs:subClassOf sba:SmartBuildingAlgorithm;
  rdfs:label "EVMPC" ;
  rdfs:comment "Model Predictive Control Algorithm to optimize the charging behaviour of Electric Vehicles for Demand Side Management. Runs every x minutes from starting time to end time as defined by the scheduler." ;
.

mpc:OptimumEVChargingSetpoints
  rdf:type owl:Class ;
  rdfs:label "OptimumEVChargingSetpoints" ;
  rdfs:comment "Model Predictive Controller generated optimum current (Ampere) setpoints for each Electric Vehicle in the EV fleet for the remaining time period of the receeding horizon." ;
  rdfs:subClassOf sba:AlgorithmOutput ;
  rdfs:subClassOf mpc:OptimumSetpoints ;
.

mpc:OptimumSetpoints
  rdf:type owl:Class ;
  rdfs:label "OptimumSetpoints" ;
  rdfs:label "Optimum setpoints generated by the optimization algorithm." ;
  rdfs:subClassOf sba:AlgorithmOutput ;
.


mpc:EVMPCModelParameters
  rdf:type owl:Class ;
  rdfs:label "EVMPCModelParameters" ;
  rdfs:comment "Parameters that described the settings corresponding to the real systems constraints or assumptions required to solve the optimization problem." ;
  rdfs:subClassOf sba:ModelParameters ;
.
